Progress on the Dafny generation target

library/src/main/java/com/aws/jverify/JVerify.java
@@ -1,13 +1,10 @@
 package com.aws.jverify;
 
-import java.util.function.BiFunction;
 import java.util.function.BiPredicate;
 import java.util.function.BooleanSupplier;
 import java.util.function.Function;
-import java.util.function.IntFunction;
 import java.util.function.IntPredicate;
 import java.util.function.Predicate;
-import java.util.function.Supplier;
 
 public class JVerify {
 
