docs/designs/equals.dfy
@@ -1,0 +1,376 @@
+// verifier
+
+
+trait Object {
+
+  ghost predicate valid()
+    requires Repr.requires()
+    reads Repr.reads(), Repr()
+    decreases Repr(), 1
+
+  ghost function Repr(): set<object> 
+    reads if this is ModifiableObject then {this as ModifiableObject} else {},
+          if this is ModifiableObject then (this as ModifiableObject).repr else {}
+  {
+    if this is ModifiableObject then (this as ModifiableObject).repr else {}
+  }
+
+  lemma ReprRequiresTrue()
+    ensures Repr.requires()
+  {}
+
+  predicate equals(other: Object): (b: bool)
+    requires valid()
+    requires other.valid()
+    reads Repr.reads(), Repr(), other.Repr.reads, other.Repr()
+    decreases Repr()
+    ensures this as Object == other ==> b
+
+  lemma equalsSymmetric(other: Object)
+    requires valid()
+    requires other.valid()
+    requires equals(other)
+    ensures other.equals(this)
+
+  method equalsImpl(other: Object) returns (b: bool)
+    requires Repr.requires()
+    requires valid()
+    requires other.Repr.requires()
+    requires other.valid()
+    ensures b == equals(other)
+
+  function getClass(): Class
+}
+
+trait ModifiableObject extends Object, object { 
+
+  var repr: set<object>
+
+  ghost predicate validComponent(component: ModifiableObject)
+    reads Repr.reads(), Repr()
+    decreases Repr(), 0
+  {
+      && this in Repr()
+      && component in Repr()
+      && component.repr <= Repr()
+      && this !in component.Repr()
+      && component.valid()
+  }
+}
+
+function JString(s: string): DString
+  requires forall i | 0 <= i < |s| :: 0 <= s[i] as int <= 65535
+{
+  JS(seq(|s|, i requires 0 <= i < |s| => s[i] as char16))
+}
+
+trait MyPair extends ModifiableObject, object {
+  var a: A
+  var b: B
+
+  method init??_MyPair(a: A, b: B)
+    modifies this
+  {
+    this.a := a;
+    this.b := b;
+  }
+
+  ghost predicate valid() 
+    requires Repr.requires()
+    reads Repr.reads(), Repr()
+    decreases Repr(), 1
+  {
+    && this in Repr()
+    && validComponent(a)
+    && validComponent(b)
+  }
+
+  predicate equals(obj: Object): (b: bool)
+    requires valid()
+    requires obj.valid()
+    reads Repr.reads, Repr(), obj.Repr.reads, obj.Repr()
+    ensures this as Object == obj ==> b
+    decreases Repr()
+  {
+    if !(obj is MyPair) then
+      false
+    else
+      var other: MyPair := obj as MyPair;
+      var result? := a.equals(other.a) && b.equals(other.b);
+      result?
+  }
+
+  method equalsImpl(obj: Object) returns (result?: bool)
+    requires Repr.requires()
+    
+    requires valid()
+    requires obj.valid()
+    ensures result? == equals(obj)
+  {
+    if !(obj is MyPair) {
+      result? := false;
+      return;
+    }
+    var other: MyPair := obj as MyPair;
+    result? := a.equals(other.a) && b.equals(other.b);
+    return;
+  }
+}
+
+class Constructable?MyPair extends MyPair {
+
+  constructor ctor?(a: A, b: B)
+
+  // predicate equals(other: Object): (b: bool)
+  //   ensures this as Object == other ==> b
+
+  lemma equalsSymmetric(other: Object)
+    requires valid()
+    requires other.valid()
+    requires equals(other)
+    ensures other.equals(this)
+  {}
+
+  function getClass(): Class
+}
+
+trait A extends ModifiableObject {
+  var f: int32
+
+  method init??_A(f: int32)
+    modifies this
+  {
+    this.f := f;
+  }
+
+  method equalsImpl(obj: Object) returns (result?: bool)
+    ensures result? == equals(obj)
+  {
+    if !(obj is A) {
+      result? := false;
+      return;
+    }
+    var other: A := obj as A;
+    result? := f == other.f;
+    return;
+  }
+}
+
+class Constructable?A extends A {
+
+  ghost predicate valid()
+    requires Repr.requires()
+    reads Repr.reads(), Repr()
+    decreases Repr(), 0
+
+  constructor ctor?(f: int32)
+
+  predicate equals(other: Object): (b: bool)
+    ensures this as Object == other ==> b
+    decreases Repr()
+
+  lemma equalsSymmetric(other: Object)
+    requires equals(other)
+    ensures other.equals(this)
+  {}
+
+  function getClass(): Class
+}
+
+trait B extends A, object {
+  var g: int32
+
+  method init??_B(f: int32, g: int32)
+    modifies this
+  {
+    init??_A(f);
+    this.g := g;
+  }
+
+  method equalsImpl(obj: Object) returns (result?: bool)
+    ensures result? == equals(obj)
+  {
+    if !(obj is B) {
+      result? := false;
+      return;
+    }
+    var other: B := obj as B;
+    result? := f == other.f && g == other.g;
+    return;
+  }
+}
+
+class Constructable?B extends B {
+  ghost predicate valid()
+
+  constructor ctor?(f: int32, g: int32)
+
+  function equals(other: Object): (b: bool)
+    decreases Repr()
+    ensures this as Object == other ==> b
+
+
+  lemma equalsSymmetric(other: Object)
+    requires equals(other)
+    ensures other.equals(this)
+  {}
+
+  function getClass(): Class
+}
+
+class Constructable?ModifiableObject extends ModifiableObject {
+
+  ghost predicate valid()
+
+  constructor ctor?()
+
+  predicate equals(other: Object): (b: bool)
+    decreases Repr()
+    ensures this as Object == other ==> b
+  {
+    other is ModifiableObject && this == other as ModifiableObject
+  }
+
+
+  lemma equalsSymmetric(other: Object)
+    requires equals(other)
+    ensures other.equals(this)
+  {}
+
+  function getClass(): Class
+
+  method equalsImpl(other: Object) returns (b: bool)
+    ensures b == equals(other)
+}
+
+trait Class extends ModifiableObject {
+
+}
+
+type nat15 = x: int16
+  | x >= 0
+
+type int16 = x: int
+  | -32768 <= x <= 32767
+
+type nat31 = x: int32
+  | x >= 0
+
+type int32 = x: int
+  | -2147483648 <= x && x <= 2147483647
+
+type nat63 = x: int64
+  | x >= 0
+
+type int64 = x: int
+  | -9223372036854775808 <= x <= 9223372036854775807
+
+type char16 = i: int
+  | 0 <= i <= 65535
+
+datatype DString extends Object = JS(elements: seq<char16>) {
+  ghost predicate valid()
+
+  function indexOf_i(c: char16): (result: int32)
+    ensures -1 <= result < |this.elements|
+    ensures result == -1 <==> forall i | 0 <= i < |this.elements| :: this.elements[i] != c
+    ensures result >= 0 && result < |this.elements| ==> this.elements[result] == c && forall j | 0 <= j && j < result :: this.elements[j] != c
+
+  function length(): int
+  {
+    |this.elements|
+  }
+
+  function charAt(x: int): char16
+    requires 0 <= x < |this.elements|
+  {
+    this.elements[x]
+  }
+
+  function isEmpty(): bool
+  {
+    this.elements == []
+  }
+
+  function concat(other: DString): DString
+  {
+    JS(this.elements + other.elements)
+  }
+
+  function substring_i(start: int): DString
+    requires start >= 0 && start <= |this.elements|
+  {
+    JS(this.elements[start..])
+  }
+
+  function substring_ii(start: int, end: int): DString
+    requires start >= 0 && start <= end && end <= |this.elements|
+  {
+    JS(this.elements[start .. end])
+  }
+
+  predicate equals(other: Object): (b: bool)
+    decreases Repr()
+    ensures this as Object == other ==> b
+  {
+    other is DString &&
+    this.elements == (other as DString).elements
+  }
+
+  lemma equalsSymmetric(other: Object)
+    requires equals(other)
+    ensures other.equals(this)
+  {}
+
+
+  function startsWith_Cjava_lang_String(other: DString): (b: bool)
+    ensures |other.elements| > |this.elements| ==> b == false
+    ensures |other.elements| <= |this.elements| && (forall i | 0 <= i < |other.elements| :: other.elements[i] == this.elements[i]) ==> b == true
+    ensures |other.elements| <= |this.elements| && (exists i | 0 <= i < |other.elements| :: other.elements[i] != this.elements[i]) ==> b == false
+
+  function getClass(): Class
+
+  method equalsImpl(other: Object) returns (b: bool)
+    ensures b == equals(other)
+}
+
+datatype DNull extends Object = DNull {
+  ghost predicate valid()
+
+  predicate equals(other: Object): (b: bool)
+    decreases Repr()
+    ensures this as Object == other ==> b
+  {
+    other is DNull
+  }
+
+  function getClass(): Class
+  method equalsImpl(other: Object) returns (b: bool)
+    ensures b == equals(other)
+
+  lemma equalsSymmetric(other: Object)
+    requires equals(other)
+    ensures other.equals(this)
+  {}
+}
+
+type byte = x
+  | 0 <= x < 256
+
+type float = real
+
+type double = real
+
+
+trait List<T> extends Object, object {
+
+  ghost const elements: seq<T>
+
+  predicate equals(obj: Object): (b: bool)
+    decreases Repr()
+    ensures this as Object == obj ==> b
+    ensures b <==>
+      && obj is List<T> 
+      && var other := obj as List<T>;
+      && elements == other.elements
+}
